Update Hoare Logic.

Coq/Coq24.v
@@ -135,3 +135,391 @@ Proof.
   auto. rewrite t_update_eq. auto.
 Qed.
 
+Theorem hoare_consequence_pre : ∀(P P' Q : Assertion) c,
+  {{P'}} c {{Q}} →
+  P ->> P' →
+  {{P}} c {{Q}}.
+Proof.
+  intros P P' Q c Hhoare Himp.
+  intros st st' Hc HP. apply (Hhoare st st').
+  assumption. apply Himp. assumption. Qed.
+
+Theorem hoare_consequence_post : ∀(P Q Q' : Assertion) c,
+  {{P}} c {{Q'}} →
+  Q' ->> Q →
+  {{P}} c {{Q}}.
+Proof.
+  intros. intros st st' Hc HP.
+  apply H0. apply (H st st').
+  auto. auto.
+Qed.
+
+Example hoare_asgn_example1 :
+  {{fun st => True}} X ::= 1 {{fun st => st X = 1}}.
+Proof.
+  apply hoare_consequence_pre
+    with (P' := (fun st => st X = 1) [X ⊢> 1]).
+  apply hoare_asgn.
+  intros st H. unfold assn_sub, t_update. simpl. reflexivity.
+Qed.
+
+Example assn_sub_example2 :
+  {{(fun st => st X < 4)}}
+  X ::= X + 1
+  {{fun st => st X < 5}}.
+Proof.
+  apply hoare_consequence_pre
+    with (P' := (fun st => st X < 5) [X ⊢> X + 1]).
+  apply hoare_asgn.
+  intros st H. unfold assn_sub, t_update. simpl. omega.
+Qed.
+
+Theorem hoare_consequence : ∀(P P' Q Q' : Assertion) c,
+  {{P'}} c {{Q'}} →
+  P ->> P' →
+  Q' ->> Q →
+  {{P}} c {{Q}}.
+Proof.
+  intros P P' Q Q' c Hht HPP' HQ'Q.
+  apply hoare_consequence_pre with (P' := P').
+  apply hoare_consequence_post with (Q' := Q').
+  assumption. assumption. assumption. Qed.
+
+Lemma assn_sub_ex1' : {{ fun st =>  st X + 1 <= 5 }} X ::= X + 1 {{ fun st => st X <= 5 }}.
+Proof.
+  eapply hoare_consequence_pre.
+  apply hoare_asgn.
+  intros st H. unfold assn_sub, t_update. simpl.
+  auto.
+Qed.
+
+Lemma assn_sub_ex2' : {{ fun st => 0 <= 3 /\ 3 <= 5 }} X ::= 3 {{ fun st => 0 <= st X /\ st X <= 5}}.
+Proof.
+  eapply hoare_consequence_pre.
+  apply hoare_asgn. intros st H.
+  unfold assn_sub, t_update.   simpl. auto.
+Qed.
+
+Theorem hoare_skip : ∀P,
+     {{P}} SKIP {{P}}.
+Proof.
+  intros P st st' H HP. inversion H. subst.
+  assumption. Qed.
+
+Theorem hoare_seq : ∀P Q R c1 c2,
+     {{Q}} c2 {{R}} →
+     {{P}} c1 {{Q}} →
+     {{P}} c1;;c2 {{R}}.
+Proof.
+  intros P Q R c1 c2 H1 H2 st st' H12 Pre.
+  inversion H12; subst.
+  apply (H1 st'0 st'); try assumption.
+  apply (H2 st st'0); assumption. Qed.
+
+Example hoare_asgn_example3 : ∀a n,
+  {{fun st => aeval st a = n}}
+  X ::= a;; SKIP
+  {{fun st => st X = n}}.
+Proof.
+  intros a n. eapply hoare_seq.
+  - apply hoare_skip.
+  - eapply hoare_consequence_pre. apply hoare_asgn.
+    intros st H. subst. reflexivity.
+Qed.
+
+Example hoare_asgn_example4 :
+  {{fun st => True}}
+  X ::= 1;; Y ::= 2
+  {{fun st => st X = 1 ∧ st Y = 2}}.
+Proof.
+  eapply hoare_seq.
+  - apply hoare_asgn.
+  - eapply hoare_consequence_pre.
+    apply hoare_asgn.
+    unfold assn_sub, t_update. simpl.
+    intros st H. auto.
+Qed.
+
+Definition swap_program : com :=
+  Z ::= X ;; X ::= Y ;; Y ::= Z.
+
+Theorem swap_exercise :
+  {{fun st => st X ≤ st Y}}
+  swap_program
+  {{fun st => st Y ≤ st X}}.
+Proof.
+  unfold swap_program.
+  eapply hoare_seq.
+  - eapply hoare_seq.
+    apply hoare_asgn.
+    apply hoare_asgn.
+  - eapply hoare_consequence_pre.
+    apply hoare_asgn.
+    unfold assn_sub, t_update.
+    simpl.
+    intros st H. auto.
+Qed.
+
+Definition bassn b : Assertion :=
+  fun st => (beval st b = true).
+
+Lemma bexp_eval_true : ∀b st,
+  beval st b = true → (bassn b) st.
+Proof.
+  intros b st Hbe.
+  unfold bassn. assumption. Qed.
+
+Lemma bexp_eval_false : ∀b st,
+  beval st b = false → ¬((bassn b) st).
+Proof.
+  intros b st Hbe contra.
+  unfold bassn in contra.
+  rewrite -> contra in Hbe. inversion Hbe. Qed.
+
+Theorem hoare_if : ∀P Q b c1 c2,
+  {{fun st => P st ∧ bassn b st}} c1 {{Q}} →
+  {{fun st => P st ∧ ¬(bassn b st)}} c2 {{Q}} →
+  {{P}} IFB b THEN c1 ELSE c2 FI {{Q}}.
+Proof.
+  intros P Q b c1 c2 HTrue HFalse st st' HE HP.
+  inversion HE; subst.
+  - apply (HTrue st st').
+    auto. split. auto. apply bexp_eval_true. auto.
+  - apply (HFalse st st').
+    auto. split. auto. apply bexp_eval_false. auto.
+Qed.
+
+Theorem if_minus_plus :
+  {{fun st => True}}
+  IFB X ≤ Y
+    THEN Z ::= Y - X
+    ELSE Y ::= X + Z
+  FI
+  {{fun st => st Y = st X + st Z}}.
+Proof.
+  eapply hoare_if.
+  - eapply hoare_consequence_pre. apply hoare_asgn.
+    unfold bassn, assn_sub, t_update. simpl.
+    intros st [_ H]. apply leb_le in H. omega.
+  - eapply hoare_consequence_pre. apply hoare_asgn.
+    unfold bassn, assn_sub, t_update. simpl.
+    intros st H. auto.
+Qed.
+
+Module If1.
+Inductive com : Type :=
+  | CSkip : com
+  | CAss : string → aexp → com
+  | CSeq : com → com → com
+  | CIf : bexp → com → com → com
+  | CWhile : bexp → com → com
+  | CIf1 : bexp → com → com.
+Notation "'SKIP'" :=
+  CSkip : imp_scope.
+Notation "c1 ;; c2" :=
+  (CSeq c1 c2) (at level 80, right associativity) : imp_scope.
+Notation "X '::=' a" :=
+  (CAss X a) (at level 60) : imp_scope.
+Notation "'WHILE' b 'DO' c 'END'" :=
+  (CWhile b c) (at level 80, right associativity) : imp_scope.
+Notation "'TEST' e1 'THEN' e2 'ELSE' e3 'FI'" :=
+  (CIf e1 e2 e3) (at level 80, right associativity) : imp_scope.
+Notation "'IF1' b 'THEN' c 'FI'" :=
+  (CIf1 b c) (at level 80, right associativity) : imp_scope.
+
+Reserved Notation "st '=[' c ']⇒' st'" (at level 40).
+Open Scope imp_scope.
+Inductive ceval : com → state → state → Prop :=
+  | E_Skip : ∀st,
+      st =[ SKIP ]⇒ st
+  | E_Ass : ∀st a1 n x,
+      aeval st a1 = n →
+      st =[ x ::= a1 ]⇒ (x !-> n ; st)
+  | E_Seq : ∀c1 c2 st st' st'',
+      st =[ c1 ]⇒ st' →
+      st' =[ c2 ]⇒ st'' →
+      st =[ c1 ;; c2 ]⇒ st''
+  | E_IfTrue : ∀st st' b c1 c2,
+      beval st b = true →
+      st =[ c1 ]⇒ st' →
+      st =[ TEST b THEN c1 ELSE c2 FI ]⇒ st'
+  | E_IfFalse : ∀st st' b c1 c2,
+      beval st b = false →
+      st =[ c2 ]⇒ st' →
+      st =[ TEST b THEN c1 ELSE c2 FI ]⇒ st'
+  | E_WhileFalse : ∀b st c,
+      beval st b = false →
+      st =[ WHILE b DO c END ]⇒ st
+  | E_WhileTrue : ∀st st' st'' b c,
+      beval st b = true →
+      st =[ c ]⇒ st' →
+      st' =[ WHILE b DO c END ]⇒ st'' →
+      st =[ WHILE b DO c END ]⇒ st''
+  | E_IF1Ture : forall st st' b c,
+      beval st b = true ->
+      st =[ c ]⇒ st' ->
+      st =[ IF1 b THEN c FI ]⇒ st'
+  | E_IF1False : forall st b c,
+      beval st b = false ->
+      st =[ IF1 b THEN c FI ]⇒ st
+  where "st '=[' c ']⇒' st'" := (ceval c st st').
+Definition hoare_triple
+           (P : Assertion) (c : com) (Q : Assertion) : Prop :=
+  ∀st st',
+       st =[ c ]⇒ st' →
+       P st →
+       Q st'.
+Notation "{{ P }} c {{ Q }}" := (hoare_triple P c Q)
+                                  (at level 90, c at next level)
+                                : hoare_spec_scope.
+Lemma hoare_if1 : forall P Q b c,
+    {{ fun st =>  P st /\ bassn b st }} c {{ Q }} -> {{ P }} (IF1 b THEN c FI) {{ fun st => P st \/ Q st}}.
+Proof.
+  intros P Q b c HTrue st st' HE HP.
+  inversion HE; subst.
+  - right. apply (HTrue st st'). auto.
+    split. auto. apply bexp_eval_true. auto.
+  - left. auto.
+Qed.
+End If1.
+
+Theorem hoare_while : ∀P b c,
+  {{fun st => P st ∧ bassn b st}} c {{P}} →
+  {{P}} WHILE b DO c END {{fun st => P st ∧ ¬(bassn b st)}}.
+Proof.
+  intros P b c Hhoare st st' He HP.
+  remember (WHILE b DO c END)%imp as wcom eqn:Heqwcom.
+  induction He;
+    try (inversion Heqwcom); subst; clear Heqwcom.
+  - (* E_WhileFalse *)
+    split. assumption. apply bexp_eval_false. assumption.
+  - (* E_WhileTrue *)
+    apply IHHe2. reflexivity.
+    apply (Hhoare st st'). assumption.
+      split. assumption. apply bexp_eval_true. assumption.
+Qed.
+
+Example while_example :
+    {{fun st => st X ≤ 3}}
+  WHILE X ≤ 2
+  DO X ::= X + 1 END
+    {{fun st => st X = 3}}.
+Proof.
+  eapply hoare_consequence_post.
+  apply hoare_while.
+  eapply hoare_consequence_pre.
+  apply hoare_asgn.
+  unfold bassn, assn_sub, assert_implies, t_update. simpl.
+    intros st [H1 H2]. apply leb_complete in H2. omega.
+  unfold bassn, assert_implies. intros st [Hle Hb].
+    simpl in Hb. destruct ((st X) <=? 2) eqn : Heqle.
+    exfalso. apply Hb; reflexivity.
+    apply leb_iff_conv in Heqle. omega.
+Qed.
+
+Theorem always_loop_hoare : ∀P Q,
+  {{P}} WHILE true DO SKIP END {{Q}}.
+Proof.
+  intros P Q.
+  apply hoare_consequence_pre with (P' := fun st : state => True).
+  eapply hoare_consequence_post.
+  apply hoare_while.
+  - apply hoare_post_true. intros. apply I.
+  - simpl. intros st [Hinv Hguard].
+    exfalso. apply Hguard. reflexivity.
+  - intros st H. constructor. Qed.
+
+Module RepeatExercise.
+Inductive com : Type :=
+  | CSkip : com
+  | CAsgn : string → aexp → com
+  | CSeq : com → com → com
+  | CIf : bexp → com → com → com
+  | CWhile : bexp → com → com
+  | CRepeat : com → bexp → com.
+
+Notation "'SKIP'" :=
+  CSkip.
+Notation "c1 ;; c2" :=
+  (CSeq c1 c2) (at level 80, right associativity).
+Notation "X '::=' a" :=
+  (CAsgn X a) (at level 60).
+Notation "'WHILE' b 'DO' c 'END'" :=
+  (CWhile b c) (at level 80, right associativity).
+Notation "'TEST' e1 'THEN' e2 'ELSE' e3 'FI'" :=
+  (CIf e1 e2 e3) (at level 80, right associativity).
+Notation "'REPEAT' e1 'UNTIL' b2 'END'" :=
+  (CRepeat e1 b2) (at level 80, right associativity).
+
+Reserved Notation "st '=[' c ']⇒' st'" (at level 40).
+Inductive ceval : state → com → state → Prop :=
+  | E_Skip : ∀st,
+      st =[ SKIP ]⇒ st
+  | E_Ass : ∀st a1 n x,
+      aeval st a1 = n →
+      st =[ x ::= a1 ]⇒ (x !-> n ; st)
+  | E_Seq : ∀c1 c2 st st' st'',
+      st =[ c1 ]⇒ st' →
+      st' =[ c2 ]⇒ st'' →
+      st =[ c1 ;; c2 ]⇒ st''
+  | E_IfTrue : ∀st st' b c1 c2,
+      beval st b = true →
+      st =[ c1 ]⇒ st' →
+      st =[ TEST b THEN c1 ELSE c2 FI ]⇒ st'
+  | E_IfFalse : ∀st st' b c1 c2,
+      beval st b = false →
+      st =[ c2 ]⇒ st' →
+      st =[ TEST b THEN c1 ELSE c2 FI ]⇒ st'
+  | E_WhileFalse : ∀b st c,
+      beval st b = false →
+      st =[ WHILE b DO c END ]⇒ st
+  | E_WhileTrue : ∀st st' st'' b c,
+      beval st b = true →
+      st =[ c ]⇒ st' →
+      st' =[ WHILE b DO c END ]⇒ st'' →
+      st =[ WHILE b DO c END ]⇒ st''
+  | E_RepeatTrue : forall b st st' c,
+      st =[ c ]⇒ st' ->
+      beval st' b = true ->
+      st =[ REPEAT c UNTIL b END ]⇒ st'
+  | E_RepeatFalse : forall st st' st'' b c,
+      st =[ c ]⇒ st' ->
+      beval st' b = false ->
+      st' =[ REPEAT c UNTIL b END ]⇒ st'' ->
+      st =[ REPEAT c UNTIL b END ]⇒ st''
+
+where "st '=[' c ']⇒' st'" := (ceval st c st').
+
+Definition hoare_triple (P : Assertion) (c : com) (Q : Assertion)
+                        : Prop :=
+  ∀st st', st =[ c ]⇒ st' → P st → Q st'.
+Notation "{{ P }} c {{ Q }}" :=
+  (hoare_triple P c Q) (at level 90, c at next level).
+
+Definition ex1_repeat :=
+  REPEAT
+    X ::= 1;;
+    Y ::= Y + 1
+  UNTIL X = 1 END.
+Theorem ex1_repeat_works :
+  empty_st =[ ex1_repeat ]⇒ (Y !-> 1 ; X !-> 1).
+Proof.
+  unfold ex1_repeat. apply E_RepeatTrue.
+  - apply E_Seq with (X !-> 1). apply E_Ass. auto.
+    apply E_Ass. auto.
+  - simpl. auto.
+Qed.
+
+Lemma hoare_repeat : forall P b c, {{ P }} c {{ P }} ->
+                                   {{ P }} (REPEAT c UNTIL b END) {{ fun st => P st /\ bassn b st}}.
+Proof.
+    intros P b c Hhoare st st' He HP.
+  remember (REPEAT c UNTIL b END)%imp as wcom eqn:Heqwcom.
+  induction He;
+    try (inversion Heqwcom); subst; clear Heqwcom.
+    - split. apply (Hhoare st st'). auto. auto.
+      apply bexp_eval_true. auto.
+    - apply IHHe2. auto. apply (Hhoare st st'). auto. auto.
+Qed.
+
+(* LEAVING Additional Exercises. *)
